removing unused file; adding an interface for Steel.PCM.Effect.Atomic

ulib/experimental/Steel.PCM.Effect.Atomic.fst
@@ -14,20 +14,11 @@
    limitations under the License.
 *)
 
-
 module Steel.PCM.Effect.Atomic
 open Steel.PCM
 open Steel.PCM.Memory
 
-let observability : Type = bool
-let observable = true
-let unobservable = false
-
-let obs_at_most_one o1 o2 : bool =
-  not (o1 && o2)
-
-let join_obs (o1:observability) (o2:observability{obs_at_most_one o1 o2}) = o1 || o2
-
+//just for fun
 let obs_pcm : pcm observability = {
   p = {
     composable = (fun x y -> ~(x==true /\ y==true));
@@ -40,118 +31,27 @@ let obs_pcm : pcm observability = {
   is_unit = (fun _ -> ())
 }
 
+let atomic_repr a opened_invariants f pre post =
+    action_except a opened_invariants pre post
 
-type atomic_repr (a:Type)
-                 (opened_invariants:inames)
-                 (g:observability)
-                 (pre:slprop)
-                 (post:a -> slprop) =
-  action_except a opened_invariants pre post
+let return a x o p = fun _ -> x
 
-let return (a:Type u#a) (x:a) (opened_invariants:inames) (p:a -> slprop u#1)
-  : atomic_repr a opened_invariants unobservable (p x) p
-  = fun _ -> x
-
-let bind (a:Type)
-         (b:Type)
-         (opened_invariants:inames)
-         (o1:observability)
-         (o2:observability{obs_at_most_one o1 o2})
-         (pre_f:slprop)
-         (post_f:a -> slprop)
-         (post_g:b -> slprop)
-         (f:atomic_repr a opened_invariants o1 pre_f post_f)
-         (g:(x:a -> atomic_repr b opened_invariants o2 (post_f x) post_g))
-  : atomic_repr b opened_invariants (join_obs o1 o2) pre_f post_g
-  = fun m0 ->
+let bind a b o o1 o2 pre_f post_f post_g f g =
+  fun m0 ->
     let x = f () in
     g x ()
 
-let subcomp (a:Type)
-            (opened_invariants:inames)
-            (o:observability)
-            (pre:slprop)
-            (post:a -> slprop)
-            (f:atomic_repr a opened_invariants o pre post)
-  : Pure (atomic_repr a opened_invariants o pre post)
-         (requires True)
-         (ensures fun _ -> True)
-  = f
-
-let if_then_else (a:Type)
-                 (opened_invariants:inames)
-                 (o:observability)
-                 (pre:slprop)
-                 (post:a -> slprop)
-                 (f:atomic_repr a opened_invariants o pre post)
-                 (g:atomic_repr a opened_invariants o pre post)
-                 (p:Type0)
-  : Type
-  = atomic_repr a opened_invariants o pre post
-
-total
-reifiable reflectable
-layered_effect {
-  SteelAtomic : a:Type
-              -> opened_invariants:inames
-              -> o:observability
-              -> pre:slprop u#1
-              -> post:(a -> slprop u#1)
-              -> Effect
-  with
-  repr = atomic_repr;
-  return = return;
-  bind = bind;
-  subcomp = subcomp;
-  if_then_else = if_then_else
-}
+let subcomp a op o pre post f = f
 
 inline_for_extraction
-let lift_pure_steel_atomic (a:Type)
-                           (opened_invariants:inames)
-                           (p:slprop)
-                           (wp:pure_wp a)
-                           (f:unit -> PURE a wp)
-  : Pure (atomic_repr a opened_invariants unobservable p (fun _ -> p))
-         (requires wp (fun _ -> True))
-         (ensures fun _ -> True)
+let lift_pure_steel_atomic a op p wp f
   = FStar.Monotonic.Pure.wp_monotonic_pure ();
     fun _ -> let x = f () in x
 
 sub_effect PURE ~> SteelAtomic = lift_pure_steel_atomic
 
-[@@warn_on_use "as_atomic_action is a trusted primitive"]
-let as_atomic_action #a (#opened_invariants:inames) (#o:observability) (#fp:slprop) (#fp': a -> slprop)
-                     (f:action_except a opened_invariants fp fp')
-  : SteelAtomic a opened_invariants o fp fp'
-  = SteelAtomic?.reflect f
-
-let new_invariant (opened_invariants:inames) (p:slprop)
-  : SteelAtomic (inv p) opened_invariants unobservable p (fun _ -> emp)
-  = SteelAtomic?.reflect (Steel.PCM.Memory.new_invariant opened_invariants p)
-
-let with_invariant (#a:Type)
-                   (#fp:slprop)
-                   (#fp':a -> slprop)
-                   (#opened_invariants:inames)
-                   (#o:observability)
-                   (#p:slprop)
-                   (i:inv p{not (i `Set.mem` opened_invariants)})
-                   (f:unit -> SteelAtomic a (Set.union (Set.singleton i) opened_invariants) o (p `star` fp) (fun x -> p `star` fp' x))
-  : SteelAtomic a opened_invariants o fp fp'
-  = SteelAtomic?.reflect (Steel.PCM.Memory.with_invariant i (reify (f())))
-
-let frame (#a:Type) (#opened_invariants:inames) (#o:observability)
-          (#pre:slprop) (#post:a -> slprop)
-          (frame:slprop)
-          ($f:unit -> SteelAtomic a opened_invariants o pre post)
-  : SteelAtomic a opened_invariants o
-                (pre `star` frame)
-                (fun x -> post x `star` frame)
-  = SteelAtomic?.reflect (Steel.PCM.Memory.frame frame (reify (f ())))
-
-let change_slprop (#opened_invariants:inames)
-                  (p q:slprop)
-                  (proof: (m:mem) -> Lemma (requires interp p m) (ensures interp q m))
-  : SteelAtomic unit opened_invariants unobservable p (fun _ -> q)
-  = SteelAtomic?.reflect (Steel.PCM.Memory.change_slprop p q proof)
+let as_atomic_action f = SteelAtomic?.reflect f
+let new_invariant i p = SteelAtomic?.reflect (Steel.PCM.Memory.new_invariant i p)
+let with_invariant i f = SteelAtomic?.reflect (Steel.PCM.Memory.with_invariant i (reify (f())))
+let frame frame f = SteelAtomic?.reflect (Steel.PCM.Memory.frame frame (reify (f ())))
+let change_slprop p q proof = SteelAtomic?.reflect (Steel.PCM.Memory.change_slprop p q proof)
